proof/correctproof/correct_step_opcode_alu64.v
@@ -7,7 +7,8 @@ From bpf.proof Require Import Clightlogic MatchState CorrectRel CommonLemma.
 
 From bpf.clight Require Import interpreter.
 
-From bpf.proof.correctproof Require Import correct_get_opcode_alu64 correct_upd_reg.
+From bpf.proof.correctproof Require Import correct_get_opcode_alu64 correct_upd_reg
+correct_upd_flag.
 (**
 Check step_opcode_alu64.
 step_opcode_alu64
@@ -117,6 +118,14 @@ Ltac correct_forward L :=
       eapply correct_statement_if_body; [prove_in_inv | destruct x ]
   end.
 
+  Lemma Cop_add : forall vl1 vl2 m,
+       Cop.sem_binary_operation (globalenv p) Cop.Oadd
+                                (Vlong vl1) Clightdefs.tulong (Vlong vl2) Clightdefs.tulong m =
+         Some (Vlong (Int64.add vl1 vl2)).
+  Proof.
+    reflexivity.
+  Qed.
+
   Instance correct_function3_step_opcode_alu64 : forall a, correct_function3 p args res f fn modifies false match_arg_list match_res a.
   Proof.
     correct_function_from_body args.
@@ -168,58 +177,104 @@ Ltac correct_forward L :=
     destruct x eqn: Halu. (**r case discussion on each alu64_instruction *)
     - (**r op_BPF_ADD64 *)
       eapply correct_statement_switch with (n:= 0).
-      + eapply correct_statement_seq_body.
-        change_app_for_statement. admit.
-Admitted.
-        eapply correct_statement_call.
-        unfold list_rel_arg,app;
-        match goal with
-        |- correct_body _ _ _ _ ?B _ ?INV
-                     _ _ _ _ =>
-          let I := fresh "INV" in
-          set (I := INV) ; simpl in I;
-          let B1 := eval simpl in B in
-            change B with B1
-        end.
-        unfold correct_body. (**r here I could not avoid, because we must first finish upd_reg *)
-        unfold correct_body.
+      + simpl.
+        eapply correct_statement_seq_body_drop.
         intros.
-        destruct (bindM _ _ _) eqn: HbindM; [| constructor].
-        destruct p0.
-        inversion HbindM; subst.
-        intros.
-        do 3 eexists.
-        repeat split.
-        forward_star.
-        simpl.
-        repeat forward_star.
-        forward_star.
-        repeat forward_star.
-        forward_star.
-        eapply step_call.
+        eapply correct_statement_seq_body_unit.
+        change_app_for_statement.
+        eapply correct_statement_call_none.
+        my_reflex.
+        my_reflex.
         reflexivity.
-        econstructor; eauto.
-        econstructor; eauto.
-        (** eval_expr e le m a vf *)
-        idtac (* TODO *) |
-        (**  eval_exprlist e le m al tyargs vargs *)
-        idtac (* TODO *) |
-        (** Genv.find_funct ge vf = Some fd *)
-        reflexivity (**r or `econstructor; eauto`, which one is better *) |
-        (** type_of_fundef fd = Tfunction tyargs tyres cconv *)
-        reflexivity
-      ].
-        forward_star.
-
-
-
-
-
-
-        eapply Smallstep.star_step; eauto.
+        typeclasses eauto.
+        unfold correct_upd_reg.match_res. intuition.
+        { unfold modifies.
+        instantiate (1:= ins_block).
+        unfold var_inv_preserve.
+        unfold match_temp_env.
+        intros.
+        inversion H1; subst; clear H1.
+        inversion H5; subst; clear H5.
+        inversion H6; subst; clear H6.
+        inversion H7; subst; clear H7.
+        inversion H8; subst; clear H8.
+        inversion H9; subst; clear H9.
+          repeat constructor;auto.
+          -
+            revert H3.
+            unfold match_elt,fst.
+            destruct (Maps.PTree.get _st le1); try congruence.
+            unfold snd.
+            intro HH ; destruct HH ; split; auto.
+            unfold correct_upd_reg.match_res in H0.
+            unfold stateM_correct in *.
+            tauto.
+        }
+        reflexivity.
+        reflexivity.
+        reflexivity.
+        reflexivity.
+        reflexivity.
+        intros.
+        change (match_temp_env ([(_opcode_alu64, Clightdefs.tuchar,
+         correct_get_opcode_alu64.match_res op_BPF_ADD64);
+        (_st, Clightdefs.tptr (Ctypes.Tstruct _bpf_state Ctypes.noattr),
+        stateM_correct tt);
+        (_dst64, Clightdefs.tulong, stateless val64_correct c);
+        (_src64, Clightdefs.tulong, stateless val64_correct c0);
+        (_dst, Clightdefs.tuint, stateless reg_correct c1);
+        (_op, Clightdefs.tuchar, stateless int8_correct c2)]) le1 st1 m1) in H; unfold INV in H.
+        get_invariant _st.
+        get_invariant _dst.
+        get_invariant _dst64.
+        get_invariant _src64.
+        destruct c5 as (c5_1 & c5_2).
+        unfold val64_correct,stateless in c5_1.
+        destruct c5_1 as (EQ & (vl1 & VL)); subst.
+        destruct c6 as (c6_1 & c6_2).
+        destruct c6_1 as (EQ & (vl2 & VL)); subst.
+        exists (v ::v0 :: Vlong (Int64.add vl1 vl2) :: nil).
+        unfold map_opt, exec_expr.
+        rewrite p0.
+        rewrite p1. rewrite p2. rewrite p3.
+        split.
+        reflexivity.
+        intros.
         simpl.
-      intros.
-      correct_forward correct_statement_seq_body.
+        intuition.
+        unfold stateless,val64_correct.
+        split; auto. eexists ; reflexivity.
+        intros.
+        eapply correct_body_id_right.
+        eapply correct_statement_seq_body_unit.
+        change_app_for_statement.
+        eapply correct_statement_call_none.
+        my_reflex.
+        my_reflex.
+        reflexivity.
+        typeclasses eauto.
+        admit.
+        admit.
+        reflexivity.
+        reflexivity.
+        reflexivity.
+        reflexivity.
+        reflexivity.
+        admit.
+        intros. destruct x1.
+        eapply correct_body_Sreturn_None.
+        unfold match_res. auto.
+        reflexivity.
+      + reflexivity.
+      + intros.
+        get_invariant _opcode_alu64.
+        unfold exec_expr.
+        rewrite p0. f_equal.
+        unfold correct_get_opcode_alu64.match_res in c3.
+        unfold opcode_alu64_correct in c3.
+        (* opcode_alu64_correct should be a mapping between opcodes and int *)
+        admit.
+      + compute. intuition congruence.
     - (**r op_BPF_SUB64 *)
     - (**r op_BPF_MUL64 *)
     - (**r op_BPF_DIV64 *)
